theories/Deduction.v
@@ -1,0 +1,304 @@
+From FormArith Require Import Definitions Lifts.
+
+Require Import Lia.
+
+
+Inductive Derivable: list formula -> formula -> Type :=
+  | RAxiom (gamma: list formula) (idx: nat):
+      Derivable gamma (nth idx gamma FTop)
+
+  | RTop_i (gamma: list formula):
+      Derivable gamma FTop
+
+  | RBot_e (gamma: list formula) (phi: formula):
+      Derivable gamma FBot -> Derivable gamma phi
+
+  | RImp_i (gamma: list formula) (phi phi': formula):
+      Derivable (phi :: gamma) phi' -> Derivable gamma (FImp phi phi')
+
+  | RImp_e (gamma: list formula) (phi phi': formula):
+      Derivable gamma phi -> Derivable gamma (FImp phi phi') -> Derivable gamma phi'
+
+  | RConj_i (gamma: list formula) (phi phi': formula):
+      Derivable gamma phi -> Derivable gamma phi' -> Derivable gamma (FConj phi phi')
+
+  | RConj_e1 (gamma: list formula) (phi phi': formula):
+      Derivable gamma (FConj phi phi') -> Derivable gamma phi
+
+  | RConj_e2 (gamma: list formula) (phi phi': formula):
+      Derivable gamma (FConj phi phi') -> Derivable gamma phi'
+
+  | RDisj_i1 (gamma: list formula) (phi phi': formula):
+      Derivable gamma phi -> Derivable gamma (FDisj phi phi')
+
+  | RDisj_i2 (gamma: list formula) (phi phi': formula):
+      Derivable gamma phi' -> Derivable gamma (FDisj phi phi')
+
+  | RDisj_e (gamma: list formula) (phi phi' phi'': formula):
+      Derivable gamma (FDisj phi phi') ->
+      Derivable (phi :: gamma) phi'' -> Derivable (phi' :: gamma) phi'' ->
+      Derivable gamma phi''
+
+  | RForAll_i (gamma: list formula) (phi: formula):
+      Derivable (context_lift 0 1 gamma) phi -> Derivable gamma (FForAll phi)
+
+  | RForAll_e (gamma: list formula) (phi: formula) (t: term):
+      Derivable gamma (FForAll phi) -> Derivable gamma (formula_subst 0 t phi)
+
+  | RExists_i (gamma: list formula) (phi: formula) (t: term):
+      Derivable gamma (formula_subst 0 t phi) -> Derivable gamma (FExists phi)
+
+  | RExists_e (gamma: list formula) (phi phi': formula):
+      Derivable gamma (FExists phi) ->
+      Derivable (phi :: context_lift 0 1 gamma) (formula_lift 0 1 phi') ->
+      Derivable gamma phi'.
+
+
+Lemma derivable_correctness (fcts: nat -> list nat -> nat) (preds: nat -> list nat -> Prop)
+    (gamma: list formula) (phi: formula):
+  Derivable gamma phi ->
+    forall (sigma: list nat),
+      (forall (idx: nat), formula_eval fcts preds sigma (nth idx gamma FTop)) ->
+        formula_eval fcts preds sigma phi.
+Proof.
+  induction 1 as
+    [ | | ? ? _ IHind |
+      (* RImp *)  ? ? ? _ IHind | ? ? ? _ IHind1 _ IHind2 |
+      (* RConj *) ? ? ? _ IHind1 _ IHind2 | ? ? ? _ IHind | ? ? ? _ IHind |
+      (* RDisj *) ? ? ? _ IHind | ? ? ? _ IHind | ? ? ? ? _ IHind1 _ IHind2 _ IHind3 |
+      (* RForAll *) ? ? _ IHind | ? ? t _ IHind |
+      (* RExists *) ? ? t _ IHind | ? ? ? _ IHind1 _ IHind2 ];
+    simpl in *; intros sigma IHtree; intros.
+
+  (* RAxiom *)
+  - apply IHtree.
+
+  (* RTop_i *)
+  - exact I.
+
+  (* RTop_e *)
+  - exfalso.
+    apply (IHind sigma).
+    apply IHtree.
+
+  (* RImp_i *)
+  - apply (IHind sigma).
+    intros [|].
+    + assumption.
+    + apply IHtree.
+
+  (* RImp_e *)
+  - apply IHind2.
+    + apply IHtree.
+    + apply IHind1.
+      apply IHtree.
+
+  (* RConj_i *)
+  - split.
+    + apply IHind1.
+      apply IHtree.
+    + apply IHind2.
+      apply IHtree.
+
+  (* RConj_e1 *)
+  - apply IHind.
+    apply IHtree.
+
+  (* RConj_e2 *)
+  - apply IHind.
+    apply IHtree.
+
+  (* RDisj_i1 *)
+  - left.
+    apply IHind.
+    apply IHtree.
+
+  (* RDisj_i2 *)
+  - right.
+    apply IHind.
+    apply IHtree.
+
+  (* RDisj_e *)
+  - destruct (IHind1 sigma IHtree).
+    + apply IHind2.
+      intros [|]; [ assumption | apply IHtree ].
+    + apply IHind3.
+      intros [|]; [ assumption | apply IHtree ].
+
+  (* RForAll_i *)
+  - apply IHind; intros n.
+    rewrite formula_lift_nth.
+    apply formula_eval_S with (sigma := nil).
+    apply IHtree.
+
+  (* RForAll_e *)
+  - replace t with (term_lift 0 0 t).
+    2: { apply term_lift_0. }
+
+    apply formula_eval_subst_lift with (sigma := nil).
+    apply IHind.
+    apply IHtree.
+
+  (* RExists_i *)
+  - exists (term_eval fcts sigma t).
+    apply formula_eval_subst_lift with (sigma := nil).
+    rewrite term_lift_0.
+    apply IHind.
+    apply IHtree.
+
+  (* RExists_e *)
+  - destruct (IHind1 sigma IHtree) as [ n ? ].
+    apply formula_eval_S with (sigma := nil) (idx := n).
+    apply IHind2.
+
+    intros [|]; [ assumption |].
+    rewrite formula_lift_nth.
+    apply formula_eval_S with (sigma := nil).
+    apply IHtree.
+Qed.
+
+Lemma derivable_weak' (gamma: list formula) (phi: formula):
+  Derivable gamma phi ->
+    forall (gamma' gamma'': list formula) (phi': formula),
+      gamma = gamma' ++ gamma'' -> Derivable (gamma' ++ phi' :: gamma'') phi.
+Proof.
+  induction 1 as
+    [ ? idx | | ? ? _ IHind |
+      (* RImp *)  ? ? ? _ IHind | ? A B _ IHind1 _ IHind2 |
+      (* RConj *) ? ? ? _ IHind1 _ IHind2 | ? A B _ IHind | ? A B _ IHind |
+      (* RDisj *) ? ? ? _ IHind | ? ? ? _ IHind | ? A B C _ IHind1 _ IHind2 _ IHind3 |
+      (* RForAll *) ? ? _ IHind | ? ? ? _ IHind |
+      (* RExists *) ? ? t _ IHind | ? t ? _ IHind1 _ IHind2 ];
+    simpl in *; intros gamma' gamma'' phi'' ->.
+
+  (* RAxiom *)
+  - destruct (PeanoNat.Nat.ltb_spec0 idx (length gamma')).
+    { generalize (RAxiom (gamma' ++ phi'' :: gamma'') idx).
+      rewrite !app_nth1; [| lia.. ].
+      intros; assumption. }
+
+    replace (nth _ _ _) with (nth (S idx) ((gamma' ++ phi'' :: nil) ++ gamma'') FTop).
+    { rewrite app_cons_nil. apply RAxiom. }
+
+    destruct (PeanoNat.Nat.ltb_spec0 (S idx) (length (gamma' ++ phi'' :: nil))) as [ Heq |].
+    { rewrite app_length in Heq; simpl in Heq.
+      lia. }
+
+    rewrite !app_nth2; [| lia.. ].
+    rewrite app_length.
+
+    f_equal.
+    replace (length (_ :: nil)) with 1 by reflexivity.
+    lia.
+
+  (* RTop_i *)
+  - apply RTop_i.
+
+  (* RTop_e *)
+  - apply RBot_e.
+    apply IHind.
+    reflexivity.
+
+  (* RImp_i *)
+   - apply RImp_i.
+     rewrite app_comm_cons.
+     apply IHind.
+     reflexivity.
+
+  (* RImp_e *)
+   - apply RImp_e with A.
+     + apply IHind1.
+       reflexivity.
+     + apply IHind2.
+       reflexivity.
+
+  (* RConj_i *)
+  - apply RConj_i.
+    + apply IHind1.
+      reflexivity.
+    + apply IHind2.
+      reflexivity.
+
+  (* RConj_e1 *)
+  - apply RConj_e1 with B.
+    apply IHind.
+    reflexivity.
+
+  (* RConj_e2 *)
+  - apply RConj_e2 with A.
+    apply IHind.
+    reflexivity.
+
+  (* RDisj_i1 *)
+  - apply RDisj_i1.
+    apply IHind.
+    reflexivity.
+
+  (* RDisj_i2 *)
+  - apply RDisj_i2.
+    apply IHind.
+    reflexivity.
+
+  (* RDisj_e *)
+  - apply RDisj_e with A B.
+    + apply IHind1.
+      reflexivity.
+    + rewrite app_comm_cons.
+      apply IHind2.
+      reflexivity.
+    + rewrite app_comm_cons.
+      apply IHind3.
+      reflexivity.
+
+  (* RForAll_i *)
+  - apply RForAll_i.
+    rewrite <- context_lift_app; simpl.
+    apply IHind.
+    rewrite context_lift_app.
+    reflexivity.
+
+  (* RForAll_e *)
+  - apply RForAll_e.
+    apply IHind.
+    reflexivity.
+
+  (* RExists_i *)
+  - apply RExists_i with t.
+    apply IHind.
+    reflexivity.
+
+  (* RExists_e *)
+  - apply RExists_e with t.
+    + apply IHind1.
+      reflexivity.
+    + rewrite <- context_lift_app; simpl.
+      rewrite app_comm_cons.
+      apply IHind2; simpl.
+      rewrite context_lift_app.
+      reflexivity.
+Defined.
+
+Lemma derivable_weak (gamma gamma': list formula) (phi phi': formula):
+  Derivable (gamma ++ gamma') phi -> Derivable (gamma ++ phi' :: gamma') phi.
+Proof.
+  intros.
+  apply (derivable_weak' (gamma ++ gamma')).
+  - assumption.
+  - reflexivity.
+Defined.
+
+Lemma derivable_weak_gamma (gamma gamma': list formula) (phi: formula):
+  Derivable gamma phi -> Derivable (gamma' ++ gamma) phi.
+Proof.
+  intros; induction gamma'; simpl.
+  { assumption. }
+
+  apply (derivable_weak nil); simpl.
+  assumption.
+Defined.
+
+Lemma derivable_weak_phi (gamma: list formula) (phi phi': formula):
+  Derivable gamma phi -> Derivable (phi' :: gamma) phi.
+Proof.
+  apply (derivable_weak nil).
+Defined.
